@prefix rdf: <http://www.w3.org/1999/02/22-rdf-syntax-ns#> .
@prefix xsd: <http://www.w3.org/2001/XMLSchema#> .
@prefix rdfs: <http://www.w3.org/2000/01/rdf-schema#> .
@prefix owl: <http://www.w3.org/2002/07/owl#> .
@prefix lens: <http://mud.cz/sw/ed#lens/> .

lens:Lens
    a rdfs:Class, owl:Class ;
    rdfs:comment "Class of lens." .

lens:BlacklistProperties
    a rdfs:Class, owl:Class ;
    rdfs:comment "Class of lens, which don't show relations with specified properties in the graph view." ;
    rdfs:subClassOf lens:Lens .

lens:WhitelistProperties
    a rdfs:Class, owl:Class ;
    rdfs:comment "Class of lens, which show only relations with specified properties in the graph view." ;
    rdfs:subClassOf lens:Lens .

[]
    a owl:AllDisjointClasses ;
    owl:members (lens:BlacklistProperties lens:WhitelistProperties ) .

lens:property
    a rdf:Property, owl:ObjectProperty ;
    rdfs:comment "Property for specifying properties for whitelisting/blacklisting." ;
    rdfs:domain lens:Lens ;
    rdfs:range rdf:Property .

lens:NotAggregateLiterals
    a rdfs:Class, owl:Class ;
    rdfs:comment "Class of lens, which don't aggregate relations with literal objects in graph nodes as is usual." ;
    rdfs:subClassOf lens:Lens .

lens:aggregatedProperty
    a rdf:Property, owl:ObjectProperty ;
    rdfs:comment "Property for specifying properties for aggregating in graph nodes." ;
    rdfs:domain lens:Lens ;
    rdfs:range rdf:Property .

