@prefix rdf: <http://www.w3.org/1999/02/22-rdf-syntax-ns#> .
@prefix xsd: <http://www.w3.org/2001/XMLSchema#> .
@prefix rdfs: <http://www.w3.org/2000/01/rdf-schema#> .
@prefix owl: <http://www.w3.org/2002/07/owl#> .
@prefix t: <http://mud.cz/sw/ed#templates/> .

t:Template
    a rdfs:Class, owl:Class ;
    rdfs:comment "Class of templates." .

t:class
    a rdf:Property, owl:ObjectProperty ;
    rdfs:comment "Property for specifying a class to which the template belongs to, as a means of classifying it in the menu for template insertion." ;
    rdfs:domain t:Template ;
    rdfs:range rdfs:Class .

t:name
    a rdf:Property, owl:ObjectProperty ;
    rdfs:comment "Property for specifying template name" ;
    rdfs:domain t:Template .

t:path
    a rdf:Property, owl:ObjectProperty ;
    rdfs:comment "Property for specifying path from the editor executable to the template RDF file." ;
    rdfs:domain t:Template .

t:variable
    a rdf:Property, owl:ObjectProperty ;
    rdfs:comment "Property for specifying an RDF node which is to be replaced by selected node on template insertion." ;
    rdfs:domain t:Template .

